\chapter{The pull-through relation}\label{app:pull-through-relation}

\begin{prop}\label{prop:pull-through-relation}
\thmtitle{Pull-through relation}
\thmstatement{
  For any non-commuting $x_1,\ld,x_n$, and $y$ for which addition, subtraction and multiplication are defined, $x_1\cd x_ny=\pr{\mp}^nyx_1\cd x_n+\sum_{k=1}^n\pr{\mp}^{n-k}x_1\cd[x_k,y]_{\pm}\cd x_n$, where $[x,y]_{\pm}\equiv xy\pm yx$.
}
\thmproof{
  The $n=1$ case follows from the definition of the commutator brackets: $xy=\mp yx+[x,y]_{\pm}$.
  Now, assume it holds for $n$ and consider the $n+1$ case.
  Since $x_1\cd x_{n+1}y=x_1\cd x_n(\mp yx_{n+1}+[x_{n+1},y]_{\pm})$, we find
  \begin{align*}
    x_1\cd x_{n+1}y
  =&\
  \mp
    \pr{
      \pr{\mp}^nyx_1\cd x_n
    +
      \sum_{k=1}^n
      \pr{\mp}^{n-k}
      x_1\cd [x_k,y]_{\pm}\cd x_n
    }
    x_{n+1}
  +
    x_1\cd x_n[x_{n+1},y]_{\pm}
  \\=&\
    \pr{\mp}^{n+1}
    yx_1\cd x_{n+1}
  +
    \sum_{k=1}^{n+1}
    \pr{\mp}^{n+1-k}
    x_1\cd[x_k,y]_{\pm}\cd x_{n+1}
  \end{align*}
  and, by induction, the result holds for all $n$.
}
\end{prop}